HUGE CHANGE! Replace VariableMapRewriter with the new MapExecutionStateVariablesDuplicator which inherits from BuilderDuplicator rather than Duplicator and so relies on an IExprBuilder to build new Expr. Dropping this into the Executor revealed a few bugs in the SimpleExprBuilder and the fragility of the lit tests (we really need to get rid of those).
There are still huge changes we need to make. We need to rip out
the existing constant folding infrastructure which is also going to
be quite invasive.

src/Symbooglix/Executor/Executor.cs
@@ -11,7 +11,7 @@ namespace Symbooglix
 
     public class Executor : Util.IYAMLWriter
     {
-        public Executor(Program program, IStateScheduler scheduler, Solver.ISolver solver)
+        public Executor(Program program, IStateScheduler scheduler, Solver.ISolver solver, IExprBuilder builder)
         { 
             this.TheProgram = program;
             StateScheduler = scheduler;
@@ -30,10 +30,12 @@ namespace Symbooglix
             AssertFilter = null;
             this.TerminationType = ExecutorTerminationType.UNKNOWN;
             HasBeenPrepared = false;
+            this.Builder = builder;
         }
 
         private IStateScheduler StateScheduler;
         private NonSymbolicDuplicator Duplicator;
+        private IExprBuilder Builder;
         public  ExecutionState CurrentState
         {
             get;
@@ -332,7 +334,7 @@ namespace Symbooglix
                 // Check The axiom can be satisfied
                 TheSolver.SetConstraints(InitialState.Constraints);
 
-                var VMR = new VariableMapRewriter(InitialState);
+                var VMR = new MapExecutionStateVariablesDuplicator(InitialState, this.Builder);
                 VMR.ReplaceGlobalsOnly = true; // The stackframe doesn't exist yet!
 
                 Expr constraint = (Expr) VMR.Visit(axiom.Expr);
@@ -777,7 +779,7 @@ namespace Symbooglix
             // We also need to rewrite so that we remove any IdentifierExpr that refer to in program
             // variables and instead replace with expressions containing symbolic variables.
             bool stillInState = true;
-            var VR = new VariableMapRewriter(CurrentState);
+            var VR = new MapExecutionStateVariablesDuplicator(CurrentState, this.Builder);
             foreach (var VariablePair in Impl.InParams.Zip(Impl.Proc.InParams))
             {
                 // Map Procedure InParams to Implementation InParams
@@ -879,7 +881,7 @@ namespace Symbooglix
 
             // Assert each requires (this might produce failing states)
             bool stillInState = true;
-            var VR = new VariableMapRewriter(CurrentState);
+            var VR = new MapExecutionStateVariablesDuplicator(CurrentState, this.Builder);
 
             // We don't need to do any of that nasty preReplacementReMap
             // stuff here because there is no implementation
@@ -970,7 +972,7 @@ namespace Symbooglix
         {
             c.GetInstructionStatistics().IncrementCovered();
 
-            var VMR = new VariableMapRewriter(CurrentState);
+            var VMR = new MapExecutionStateVariablesDuplicator(CurrentState, this.Builder);
 
             // FIXME: The variables attached to the procedure are not the same object instances
             // used for the procedure. Setup the mapping. Eurgh.. Boogie you suck!
@@ -1058,7 +1060,7 @@ namespace Symbooglix
             c.GetInstructionStatistics().IncrementCovered();
 
             int index=0;
-            VariableMapRewriter r = new VariableMapRewriter(CurrentState);
+            var r = new MapExecutionStateVariablesDuplicator(CurrentState, this.Builder);
             Dictionary<Variable, Expr> storedAssignments = new Dictionary<Variable, Expr>();
 
             // FIXME: Should we zip asSimpleAssignCmd lhs and rhs instead?
@@ -1126,7 +1128,7 @@ namespace Symbooglix
             }
 
             HandleBreakPoints(c);
-            VariableMapRewriter r = new VariableMapRewriter(CurrentState);
+            var r = new MapExecutionStateVariablesDuplicator(CurrentState, this.Builder);
             var dupAndrw = (Expr) r.Visit(c.Expr);
 
             if (UseConstantFolding)
@@ -1347,7 +1349,7 @@ namespace Symbooglix
             c.GetInstructionStatistics().IncrementCovered();
 
             HandleBreakPoints(c);
-            VariableMapRewriter r = new VariableMapRewriter(CurrentState);
+            var r = new MapExecutionStateVariablesDuplicator(CurrentState, this.Builder);
             var dupAndrw = (Expr) r.Visit(c.Expr);
 
             if (UseConstantFolding)
@@ -1413,7 +1415,7 @@ namespace Symbooglix
             // so it should be executed normally.
             // If the Expr is not null then it is the rewritten expression
             // from an assume instruction that should be added to the constraints
-            var remapper = new VariableMapRewriter(CurrentState);
+            var remapper = new MapExecutionStateVariablesDuplicator(CurrentState, this.Builder);
             foreach (var block in c.labelTargets)
             {
                 LookAheadInfo info;
@@ -1564,7 +1566,7 @@ namespace Symbooglix
             c.GetInstructionStatistics().IncrementCovered();
 
             var args = new List<Expr>();
-            var reWritter = new VariableMapRewriter(CurrentState);
+            var reWritter = new MapExecutionStateVariablesDuplicator(CurrentState, this.Builder);
 
             // Find corresponding implementation
             Implementation impl = null;
