test_programs/basic/symbolic/bv_straight_assume_feasible.bpl
@@ -3,8 +3,8 @@
 procedure main(p1:int, p2:bv8) returns (r:bv8);
 
 // Bitvector functions
-function {:bvbuiltin "bvadd"} bv8add(bv8,bv8) returns(bv8);
-function {:bvbuiltin "bvugt"} bv8ugt(bv8,bv8) returns(bool);
+function {:bvbuiltin "bvadd"} BVADD8(bv8,bv8) returns(bv8);
+function {:bvbuiltin "bvugt"} BVUGT8(bv8,bv8) returns(bool);
 
 var g:bv8;
 
@@ -12,12 +12,12 @@ implementation main(p1:int, p2:bv8) returns (r:bv8)
 {
     var a:bv8;
     var b:bv8;
-    // CHECK: Assignment : r := bv8add\(~sb_a_0, ~sb_b_0\)
-    r := bv8add(a,b);
-    // CHECK: Assume : bv8add\(~sb_a_0, ~sb_b_0\) == 1bv8
+    // CHECK: Assignment : r := BVADD8\(~sb_a_0, ~sb_b_0\)
+    r := BVADD8(a,b);
+    // CHECK: Assume : BVADD8\(~sb_a_0, ~sb_b_0\) == 1bv8
     assume  r == 1bv8;
-    // CHECK: Assert : bv8ugt\(bv8add\(~sb_a_0, ~sb_b_0\), 0bv8\)
-    assert bv8ugt(r, 0bv8); // This is feasible so we should carry on executing
+    // CHECK: Assert : BVUGT8\(BVADD8\(~sb_a_0, ~sb_b_0\), 0bv8\)
+    assert BVUGT8(r, 0bv8); // This is feasible so we should carry on executing
     // CHECK: Assert : true
     assert true;
 }
