test_programs/basic/concrete/bv_straight.bpl
@@ -17,7 +17,7 @@ implementation main(p1:int, p2:bv8) returns (r:bv8)
     // CHECK-L: ${CHECKFILE_ABS_PATH}:${LINE:+1}: [Cmd] b := 2bv8;
     b := 2bv8;
     // CHECK-L: ${CHECKFILE_ABS_PATH}:${LINE:+2}: [Cmd] r := bv8add(a, b);
-    // CHECK-L: Assignment : r := bv8add(1bv8, 2bv8)
+    // CHECK-L: Assignment : r := BVADD8(1bv8, 2bv8)
     r := bv8add(a,b);
     assert bv8ugt(r, 0bv8);
 }
